@prefix tree: <https://w3id.org/tree#> .
@prefix tiles: <https://w3id.org/tree#> .
@prefix cc: <http://creativecommons.org/ns#> .
@prefix dct: <http://purl.org/dc/terms/> .
@prefix foaf: <http://xmlns.com/foaf/0.1/> .
@prefix gsp: <http://www.opengis.net/ont/geosparql#> .
@prefix locn: <http://www.w3.org/ns/locn#> .
@prefix owl: <http://www.w3.org/2002/07/owl#> .
@prefix prov: <http://www.w3.org/ns/prov#> .
@prefix rdf: <http://www.w3.org/1999/02/22-rdf-syntax-ns#> .
@prefix rdfs: <http://www.w3.org/2000/01/rdf-schema#> .
@prefix schema: <http://schema.org/> .
@prefix sh: <http://www.w3.org/ns/shacl#> .
@prefix voaf: <http://purl.org/vocommons/voaf#> .
@prefix vs: <http://www.w3.org/2003/06/sw-vocab-status/ns#> .
@prefix wdrs: <http://www.w3.org/2007/05/powder-s#> .
@prefix xhtm: <http://www.w3.org/1999/xhtml> .
@prefix xml: <http://www.w3.org/XML/1998/namespace> .
@prefix xsd: <http://www.w3.org/2001/XMLSchema#> .
@prefix hydra: <http://www.w3.org/ns/hydra/core#>.


tree: a foaf:Document ;
      foaf:primaryTopic tree:Ontology;
      cc:license <http://creativecommons.org/licenses/by/4.0/>;
      dct:creator <https://pietercolpaert.be/#me>, <http://www.rubensworks.net/#me>.

<https://pietercolpaert.be/#me> foaf:name "Pieter Colpaert"; foaf:mbox "pieter.colpaert@ugent.be".

<http://www.rubensworks.net/#me> foaf:name "Ruben Taelman" .

tree:Ontology a owl:Ontology ;
              rdfs:label "Tree Ontology"@en;
              rdfs:comment "Ontology for describing tree-like relations between hypermedia documents."@en.

######## Classes

tree:Node a rdfs:Class ;
          rdfs:label "Node"@en;
          rdfs:comment "A tree:Node is a node that contains a link to other dereferenceable resources"@en . #, may contain the actual data (as part of a named graph, or using the predicate hydra:member)."@en.

tree:ChildRelation a rdfs:Class ;
                   rdfs:label "Child Relation"@en ;
                   rdfs:comment "A class describing the relation between a parent and a child"@en.


tree:StringCompletesRelation a rdfs:Class ;
                             rdfs:subClassOf tree:ChildRelation ;
                             rdfs:label "String Completes Relation"@en;
                             rdfs:comment "The parent value needs to be concatenated with this nodeâ€™s value"@en .

tree:GreaterThanRelation a rdfs:Class ;
                         rdfs:subClassOf tree:ChildRelation ;
                         rdfs:label "Greater Than Relation"@en ;
                         rdfs:comment "The child is greater than the value. For string comparison, this relation can refer to a comparison configuration."@en .
                         
tree:GreaterOrEqualThanRelation  a rdfs:Class ;
                                 rdfs:subClassOf tree:ChildRelation ;
                                 rdfs:label "Greater or Equal Than Relation"@en .
tree:LesserThanRelation a rdfs:Class ;
                        rdfs:subClassOf tree:ChildRelation ;
                        rdfs:label "Lesser Than Relation"@en .
                        
tree:LesserOrEqualThanRelation a rdfs:Class ;
                               rdfs:subClassOf tree:ChildRelation ;
                               rdfs:label "Lesser or Equal than Relation"@en .
                               
tree:EqualThanRelation a rdfs:Class ;
                       rdfs:subClassOf tree:ChildRelation ;
                       rdfs:label "Equal Than Relation"@en .

tree:GeospatiallyContainsRelation  a rdfs:Class ;
                                   rdfs:subClassOf tree:ChildRelation ;
                                   rdfs:label "Geospatially Contains Relation"@en;
                                   rdfs:comment "For semantics, see [DE-9IM](https://en.wikipedia.org/wiki/DE-9IM))"@en.
                                   
tree:InBetweenRelation a rdfs:Class ;
                       rdfs:subClassOf tree:ChildRelation ;
                       rdfs:label "In Between Relation"@en ;
                       rdfs:comment "For comparing intervals: the child interval is inbetween the parent interval"@en .


######## Properties

tree:childRelation a rdf:Property ;
                   rdfs:label "Relation to child"@en;
                   rdfs:comment "Links a node with a child through a child relation class."@en;
                   rdfs:domain tree:Node;
                   rdfs:range tree:ChildRelation.

tree:child a rdf:Property ;
           rdfs:label "Child"@en;
           rdfs:comment "The specific child or children that follow a childRelation"@en;
           rdfs:domain tree:ChildRelation;
           rdfs:range tree:Node.

tree:value a rdf:Property ;
           rdfs:label "Value"@en ;
           rdfs:comment "The value this node holds in the tree. This value can be strings, integers, intervals, WKT strings, etc. This value should not be used in end-user interfaces."@en;
           rdfs:domain tree:Node .


###### Properties for the Tiles ontology
###### Mind that tiles prefix is just a synonym for the tree prefix

tiles:zoom a rdf:Property ;
           rdfs:label "Zoom level"@en;
           rdfs:comment "The zoom level of the tile cfr. OSM convention"@en;
           rdfs:isDefinedBy <https://wiki.openstreetmap.org/wiki/Slippy_map_tilenames> ;
           rdfs:domain tiles:Node;
           rdfs:range xsd:float.

tiles:longitudeTile a rdf:Property ;
           rdfs:label "The X tile number"@en;
           rdfs:comment "The X tile number from longitude cfr. OSM convention"@en;
           rdfs:isDefinedBy <https://wiki.openstreetmap.org/wiki/Slippy_map_tilenames> ;
           rdfs:domain tiles:Node;
           rdfs:range xsd:float.

tiles:latitudeTile a rdf:Property ;
           rdfs:label "The Y tile number"@en;
           rdfs:comment "The Y tile number from latitude cfr. OSM convention"@en;
           rdfs:isDefinedBy <https://wiki.openstreetmap.org/wiki/Slippy_map_tilenames> ;
           rdfs:domain tiles:Node;
           rdfs:range xsd:float.