@prefix tree: <https://w3id.org/tree#> .
@prefix cc: <http://creativecommons.org/ns#> .
@prefix dct: <http://purl.org/dc/terms/> .
@prefix foaf: <http://xmlns.com/foaf/0.1/> .
@prefix gsp: <http://www.opengis.net/ont/geosparql#> .
@prefix locn: <http://www.w3.org/ns/locn#> .
@prefix owl: <http://www.w3.org/2002/07/owl#> .
@prefix prov: <http://www.w3.org/ns/prov#> .
@prefix rdf: <http://www.w3.org/1999/02/22-rdf-syntax-ns#> .
@prefix rdfs: <http://www.w3.org/2000/01/rdf-schema#> .
@prefix schema: <http://schema.org/> .
@prefix sh: <http://www.w3.org/ns/shacl#> .
@prefix voaf: <http://purl.org/vocommons/voaf#> .
@prefix vs: <http://www.w3.org/2003/06/sw-vocab-status/ns#> .
@prefix wdrs: <http://www.w3.org/2007/05/powder-s#> .
@prefix xhtm: <http://www.w3.org/1999/xhtml> .
@prefix xml: <http://www.w3.org/XML/1998/namespace> .
@prefix xsd: <http://www.w3.org/2001/XMLSchema#> .
@prefix hydra: <http://www.w3.org/ns/hydra/core#>.


tree: a foaf:Document ;
      foaf:primaryTopic tree:Ontology;
      cc:license <http://creativecommons.org/licenses/by/4.0/>;
      dct:creator <https://pietercolpaert.be/#me>.

<https://pietercolpaert.be/#me> foaf:name "Pieter Colpaert"; foaf:mbox "pieter.colpaert@ugent.be".

tree:Ontology a owl:Ontology ;
              rdfs:label "Tree Ontology"@en;
              rdfs:comment "Ontology for describing tree-like relations between hypermedia documents."@en.

######## Classes

tree:Node a rdfs:Class ;
          rdfs:label "Node"@en;
          rdfs:comment "A tree:Node is a node that may contain links to other dereferenceable resources, may contain the actual data (as part of a named graph, or using the predicate hydra:member)."@en.

tree:ChildRelation a redfs:Class ;
                   rdfs:label "Child Relation"@en ;
                   rdfs:comment "A class describing the relation between a parent and a child"@en.


######## Properties

tree:childRelation a rdf:Property ;
                   rdfs:label "Relation to child"@en;
                   rdfs:comment "Links a node with a child through a child relation class."@en;
                   rdfs:domain tree:Node;
                   rdfs:range tree:ChildRelation.

tree:child a rdf:Property ;
           rdfs:label "Child"@en;
           rdfs:comment "The specific child or children that follow a childRelation"@en;
           rdfs:domain tree:ChildRelation;
           rdfs:range tree:Node.

tree:parent a rdf:Property ;
            rdfs:label "Parent"@en;
            rdfs:comment "The object is the parent node of the subject. Use tree:child predicate for describing trees."@en;
            rdfs:domain tree:Node;
            rdfs:range tree:Node.

tree:relationToParentValue a rdf:Property ;
                           rdfs:label "Relation to Parent Value"@en ;
                           rdfs:comment "The relation this node’s value has to the node of its parent."@en;
                           rdfs:domain tree:Node.

tree:value a rdf:Property ;
           rdfs:label "Value"@en ;
           rdfs:comment "The value this node holds in the tree. This value can be strings, integers, intervals, WKT strings, etc. This value should not be used in end-user interfaces."@en;
           rdfs:domain tree:Node .

tree:stringCompletes a rdf:Property ;
                     rdfs:label "String Completes"@en ;
                     rdfs:comment "The subject’s string value needs to be string concatenated with the object entity’s value"@en.

tree:href a rdf:Property ;
          rdfs:label "Reference"@en;
          rdfs:comment "When a client wants to process this node, first this href needs to be dereferenced."@en;
          rdfs:domain tree:Node;
          rdfs:range hydra:Resource.